Core.v
@@ -6,9 +6,18 @@ Class Serializer A :=
   {
     serialize: A -> (list bool);
     deserialize: list bool -> option (A * list bool);
-    Serialize_reversible: forall (x: A) (bin: list bool),
+    deserialize_preserves_input: forall (x: A) (bin: list bool),
                             deserialize ((serialize x) ++ bin) = Some (x, bin)
   }.
+
+Lemma Serialize_reversible:
+  forall (A: Type) (serializer: Serializer A) (x: A),
+    deserialize (serialize x) = Some(x, nil).
+Proof.
+  intros.
+  rewrite <- deserialize_preserves_input.
+  rewrite app_nil_r. reflexivity.
+Qed.
 
 Definition bool_serialize (a: bool) : list bool :=
   a :: nil.
@@ -19,7 +28,7 @@ Definition bool_deserialize (bin : list bool) : option (bool * list bool) :=
     | h :: t => Some (h, t)
   end.
 
-Lemma bool_serialize_reversible: forall (x: bool) (bin: list bool),
+Lemma bool_deserialize_preserves_input: forall (x: bool) (bin: list bool),
                                    bool_deserialize ((bool_serialize x) ++ bin) = Some (x, bin).
 Proof.
   intros; simpl.
@@ -30,14 +39,14 @@ Instance Bool_Serializer: Serializer bool :=
   {
     serialize := bool_serialize;
     deserialize := bool_deserialize;
-    Serialize_reversible := bool_serialize_reversible
+    deserialize_preserves_input := bool_deserialize_preserves_input
   }.
 
 Instance Nat_Serializer : Serializer nat :=
   {
     serialize := uleb128_encode;
     deserialize := uleb128_decode;
-    Serialize_reversible := uleb128_decode_encode
+    deserialize_preserves_input := uleb128_decode_encode
   }.
 
 Definition ascii_serialize (a : ascii) : list bool :=
@@ -49,17 +58,17 @@ Definition ascii_deserialize (bin : list bool) : option (ascii * list bool) :=
     | Some (n, rest) => Some (ascii_of_nat n, rest)
   end.
 
-Lemma ascii_serialize_reversible : forall a bin,
+Lemma ascii_deserialize_preserves_input : forall a bin,
     ascii_deserialize (ascii_serialize a ++ bin) = Some (a, bin).
 Proof.
   unfold ascii_deserialize, ascii_serialize.
   intros a bin.
-  now rewrite Serialize_reversible, ascii_nat_embedding.
+  now rewrite deserialize_preserves_input, ascii_nat_embedding.
 Qed.
 
 Instance Ascii_Serializer : Serializer ascii :=
   {
     serialize := ascii_serialize;
     deserialize := ascii_deserialize;
-    Serialize_reversible := ascii_serialize_reversible
+    deserialize_preserves_input := ascii_deserialize_preserves_input
   }.
