Extra.v
@@ -1,7 +1,9 @@
+Require Import StructTact.StructTactics.
 Require Import Ascii.
 Require Import String.
 Require Import List.
-Require Import Cheerios.Types.
+Require Import ZArith.
+Require Import Cheerios.Core.
 Require Import Cheerios.Combinators.
 
 Fixpoint string_to_list s :=
@@ -32,11 +34,43 @@ Definition string_deserialize bin : option (string * list bool) :=
     | Some (cs, rest) => Some (list_to_string cs, rest)
   end.
 
-Lemma string_serialize_reversible : forall s bin,
+Lemma string_deserialize_preserves_input : forall s bin,
     string_deserialize (string_serialize s ++ bin) = Some (s, bin).
 Proof.
   unfold string_deserialize, string_serialize.
   intros s bin.
-  rewrite Serialize_reversible.
+  rewrite deserialize_preserves_input.
   now rewrite string_to_list_to_string.
 Qed.
+
+Definition Z_to_nat (z : Z) : nat := 2 * (Z.abs_nat z) + Nat.b2n (0 <=? z)%Z.
+
+Definition nat_to_Z (n : nat) : Z :=
+  let abs := Z.of_nat (Nat.div2 n)
+  in
+  if Nat.odd n
+  then abs
+  else Z.opp abs.
+
+Lemma odd_b2n :
+  forall b, Nat.odd (Nat.b2n b) = b.
+Proof.
+  destruct b; auto.
+Qed.
+
+Lemma Z_to_nat_inverse :
+  forall z, nat_to_Z (Z_to_nat z) = z.
+Proof.
+  unfold nat_to_Z, Z_to_nat.
+  intros z.
+  rewrite Nat.div2_div, plus_comm, Nat.add_b2n_double_div2, Zabs2Nat.id_abs.
+  rewrite Nat.odd_add_mul_2, odd_b2n.
+  break_if.
+  - apply Z.leb_le in Heqb.
+    now rewrite Z.abs_eq by omega.
+  - apply Z.leb_gt in Heqb.
+    destruct (Z.abs_spec z); intuition.
+Qed.
+
+Instance Z_Serializer : Serializer Z :=
+  To_From_Serializer Nat_Serializer _ _ Z_to_nat_inverse.
